x

src/add_multiply.v
@@ -3,63 +3,75 @@ From stdpp Require Import fin finite.
 From research Require Import bit circuit multiplier fifo regfile.
 
 Inductive Instr :=
-| Add (rd rs1 rs2 : Bit 5)
-| Addi (rd rs1 : Bit 5) (imm : Bit 8)
-| Mul (rd rs1 rs2 : Bit 5)
-| Nop
-| Unknown.
+| Add (rd rs1 rs2 : Bit 3)
+| Addi (rd rs1 : Bit 3) (imm : Bit 8)
+| Muli (rd : Bit 3) (imm : Bit 8) (rs2 : Bit 3)
+| Nop.
 
 Instance defaultInstr : Default Instr := Nop.
 
-Inductive method :=
+Inductive Method :=
 | DeqIReq
 | EnqIResp (resp : Instr)
 | Rule.
 
-Inductive state :=
+Inductive State :=
 | State__Fetch
 | State__Decode
 | State__Execute.
 
-Inductive implLeakage :=
+Inductive ImplLeakage :=
 | Impl__Pc (l : Bit 32)
 | Impl__Add
 | Impl__Nop
 | Impl__Mul (a : Bit 8).
 
-Instance state__EqDecision : EqDecision state.
+Inductive SpecInstr :=
+| SAdd
+| SAddi
+| SMul (imm : Bit 8)
+| SNop.
+
+Instance defaultSpecInstr : Default SpecInstr := SNop.
+
+Inductive SpecLeakage :=
+| Spec__DeqIReq
+| Spec__EnqIResp (resp : SpecInstr)
+| Spec__Rule.
+
+Instance eqDecisionState : EqDecision State.
 Proof.
   solve_decision.
 Defined.
 
 Inductive DInstr :=
-| DAdd (rd : Bit 5) (v1 v2 : Bit 8)
-| DMul (rd : Bit 5) (v1 v2 : Bit 8)
+| DAdd (rd : Bit 3) (v1 v2 : Bit 8)
+| DMul (rd : Bit 3) (v1 v2 : Bit 8)
 | DNop.
 
 Instance defaultDInstr : Default DInstr := DNop.
 
 Record AddMultiply :=
   { addMultiplyM        : Multiplier
-  ; addMultiplyRf       : RegFile 8 5
+  ; addMultiplyRf       : RegFile 8 3
   ; addMultiplyPc       : Bit 32
   ; addMultiplyFromImem : Fifo Instr
   ; addMultiplyToImem   : Fifo (Bit 32)
   ; addMultiplyDInstr   : Fifo DInstr
-  ; addMultiplySt       : state
-  ; addMultiplyTrace    : list implLeakage
+  ; addMultiplySt       : State
+  ; addMultiplyTrace    : list ImplLeakage
   }.
 
 Definition mkAddMultiply :=
   {|
     addMultiplyM         := mkMultiplier;
     addMultiplyRf        := mkRegFile;
-    addMultiplyPc        := 0%bv;
+    addMultiplyPc        := δ;
     addMultiplyFromImem  := mkFifo;
     addMultiplyToImem    := mkFifo;
     addMultiplyDInstr    := mkFifo;
     addMultiplySt        := State__Fetch;
-    addMultiplyTrace     := []
+    addMultiplyTrace     := δ
   |}.
 
 Definition addMultiplyFetching st :=
@@ -95,13 +107,11 @@ Definition addMultiplyFetch :=
 Definition addMultiplyDecode :=
   guard
     {{ addMultiplyDecoding }}
-    {{ let%read d2e      := addMultiplyDInstr in
-       let%read rf       := addMultiplyRf in
+    {{ let%read rf       := addMultiplyRf in
        let%read instr    := fifoFirst ∘ addMultiplyFromImem in
        let%call _        := fifoDeq on addMultiplyFromImem in
        match instr with
-       | Nop
-       | Unknown =>
+       | Nop =>
            let%call  _ := fifoEnq DNop on addMultiplyDInstr in
            let%write _ := State__Execute on addMultiplySt in
            pass
@@ -111,8 +121,8 @@ Definition addMultiplyDecode :=
            let%call _ := fifoEnq (DAdd rd v1 v2) on addMultiplyDInstr in
            let%write _ := State__Execute on addMultiplySt in
            pass
-       | Mul rd rs1 rs2 =>
-           let v1 := regFileSub rs1 rf in
+       | Muli rd imm rs2 =>
+           let v1 := imm in
            let v2 := regFileSub rs2 rf in
            let%call _ := fifoEnq (DMul rd v1 v2) on addMultiplyDInstr in
            let%write _ := State__Execute on addMultiplySt in
@@ -201,76 +211,299 @@ Instance addMultiplyCircuit : Circuit :=
     circuitTrace := addMultiplyTrace
   |}.
 
-Section example.
-  Definition x0 := 5`0%bv.
-  Definition x1 := 5`1%bv.
-  Definition x2 := 5`2%bv.
-  Definition x3 := 5`3%bv.
-  Definition x4 := 5`4%bv.
-  Definition x5 := 5`5%bv.
-  Definition x6 := 5`6%bv.
-  Definition x7 := 5`7%bv.
-  Definition x8 := 5`8%bv.
+Record AddMultiplySpec :=
+  { addMultiplySpecM        : MultiplierSpec
+  ; addMultiplySpecPc       : Bit 32
+  ; addMultiplySpecFromImem : Fifo SpecInstr
+  ; addMultiplySpecToImem   : Fifo (Bit 32)
+  ; addMultiplySpecDInstr   : Fifo SpecInstr
+  ; addMultiplySpecSt       : State
+  ; addMultiplySpecTrace    : list ImplLeakage
+  }.
 
-  (* Execute a single instruction until completion *)
-  Definition executeOneInstr (fuel : nat) (instr : Instr) (st : AddMultiply) : AddMultiply :=
-    (* Fetch stage: send PC to instruction memory *)
-    let st1 := circuitSteps addMultiplyCircuit [Rule; DeqIReq; EnqIResp instr] st in
-    (* Decode stage *)
-    let st2 := circuitStep addMultiplyCircuit Rule st1 in
-    (* Execute stage - may take multiple cycles *)
-    let fix executeUntilFetch (fuel : nat) (st : AddMultiply) : AddMultiply :=
-      match fuel with
-      | 0 => st
-      | S fuel' =>
-          let st' := circuitStep addMultiplyCircuit Rule st in
-          if bool_decide (st'.(addMultiplySt) = State__Fetch) then st'
-          else executeUntilFetch fuel' st'
-      end
-    in
-    executeUntilFetch fuel st2.
+Definition mkAddMultiplySpec :=
+  {|
+    addMultiplySpecM         := mkMultiplierSpec;
+    addMultiplySpecPc        := δ;
+    addMultiplySpecFromImem  := mkFifo;
+    addMultiplySpecToImem    := mkFifo;
+    addMultiplySpecDInstr    := mkFifo;
+    addMultiplySpecSt        := State__Fetch;
+    addMultiplySpecTrace     := δ
+  |}.
 
-  (* Execute instructions with fuel *)
-  Fixpoint execute (instrs : list Instr) (st : AddMultiply) : AddMultiply :=
-    match instrs with
-    | [] => st
-    | instr :: instrs' =>
-        let st' := executeOneInstr 100 instr st in
-        execute instrs' st'
-    end.
+Definition addMultiplySpecFetching st :=
+  bool_decide (st.(addMultiplySpecSt) = State__Fetch).
 
-  (* Notation for RISC-V-like instructions *)
-  Declare Scope asm_scope.
-  Delimit Scope asm_scope with asm.
+Definition addMultiplySpecDecoding st :=
+  bool_decide (st.(addMultiplySpecSt) = State__Decode).
 
-  Notation "'li' rd , imm" := (Addi rd 5`0 imm)%bv (at level 0) : asm_scope.
-  Notation "'mv' rd , rs" := (Addi rd rs 0)%bv (at level 0) : asm_scope.
-  Notation "'addi' rd , rs1 , imm" := (Addi rd rs1 imm)%bv (at level 0) : asm_scope.
-  Notation "'add' rd , rs1 , rs2" := (Add rd rs1 rs2)%bv (at level 0) : asm_scope.
-  Notation "'mul' rd , rs1 , rs2" := (Mul rd rs1 rs2)%bv (at level 0) : asm_scope.
-  Notation "'nop'" := Nop (at level 0) : asm_scope.
-  Notation "'unk'" := Unknown (at level 0) : asm_scope.
+Definition addMultiplySpecExecuting st :=
+  bool_decide (st.(addMultiplySpecSt) = State__Execute).
 
-  Local Open Scope asm_scope.
+Definition addMultiplySpecDeqIReq :=
+  {{ let%call _ := fifoDeq on addMultiplySpecToImem in
+     pass
+  }}.
 
-  Example ex1 := [
-      li x1, 127;
-      li x2, 1;
-      mul x3, x1, x2;
-      nop;
-      nop;
-      nop;
-      add x4, x3, x3
-    ].
+Definition addMultiplySpecEnqIResp instr :=
+  {{ let%call _ := fifoEnq instr on addMultiplySpecFromImem in
+     pass
+  }}.
 
-  Eval vm_compute in (execute ex1 mkAddMultiply).
+Definition addMultiplySpecFetch :=
+  guard
+    {{ addMultiplySpecFetching }}
+    {{ let%read pc := addMultiplySpecPc in
+       let%write _ := State__Decode on addMultiplySpecSt in
+       let%call _ := fifoEnq pc on addMultiplySpecToImem in
+       pass
+    }}.
 
-  Example ex2 := [
-      li x1, 15;
-      li x2, 30;
-      add x8, x1, x2;
-      mv x3, x8
-    ].
+Definition addMultiplySpecDecode :=
+  guard
+    {{ addMultiplySpecDecoding }}
+    {{ let%read instr    := fifoFirst ∘ addMultiplySpecFromImem in
+       let%call _        := fifoDeq on addMultiplySpecFromImem in
+       let%call _        := fifoEnq instr on addMultiplySpecDInstr in
+       let%write _       := State__Execute on addMultiplySpecSt in
+       pass
+    }}.
 
-  Eval vm_compute in (execute ex2 mkAddMultiply).
-End example.
+Definition addMultiplySpecExecuteAdd :=
+  {{ let%read pc := addMultiplySpecPc in
+     let%call _ := fifoDeq on addMultiplySpecDInstr in
+     let%write _ := State__Fetch on addMultiplySpecSt in
+     let%modify _ := cons (Impl__Pc pc) on addMultiplySpecTrace in
+     let%modify _ := cons Impl__Add on addMultiplySpecTrace in
+     let%modify _ := fun pc => (pc `+Z` 4)%bv on addMultiplySpecPc in
+     pass
+  }}.
+
+Definition addMultiplySpecExecuteNop :=
+  {{ let%read pc := addMultiplySpecPc in
+     let%call _ := fifoDeq on addMultiplySpecDInstr in
+     let%write _ := State__Fetch on addMultiplySpecSt in
+     let%modify _ := cons (Impl__Pc pc) on addMultiplySpecTrace in
+     let%modify _ := cons Impl__Nop on addMultiplySpecTrace in
+     let%modify _ := fun pc => (pc `+Z` 4)%bv on addMultiplySpecPc in
+     pass
+  }}.
+
+Definition addMultiplySpecExecuteMul v1 :=
+  {{ let%read pc := addMultiplySpecPc in
+     let%read st := multiplierSpecSt ∘ addMultiplySpecM in
+     match st with
+     | State__Empty =>
+         let%call _ := multiplierSpecEnq v1 on addMultiplySpecM in
+         pass
+     | State__Busy =>
+         let%call _ := multiplierSpecRule on addMultiplySpecM in
+         pass
+     | State__Full =>
+         let%call _ := multiplierSpecDeq on addMultiplySpecM in
+         let%call _ := fifoDeq on addMultiplySpecDInstr in
+         let%write _ := State__Fetch on addMultiplySpecSt in
+         let%modify _ := cons (Impl__Pc pc) on addMultiplySpecTrace in
+         let%modify _ := cons (Impl__Mul v1) on addMultiplySpecTrace in
+         let%modify _ := fun pc => (pc `+Z` 4)%bv on addMultiplySpecPc in
+         pass
+     end
+  }}.
+
+Definition addMultiplySpecExecute :=
+  guard
+    {{ addMultiplySpecExecuting }}
+    {{ let%read instr := fifoFirst ∘ addMultiplySpecDInstr in
+       match instr with
+       | SAddi | SAdd => addMultiplySpecExecuteAdd
+       | SMul v1 => addMultiplySpecExecuteMul v1
+       | SNop => addMultiplySpecExecuteNop
+       end
+    }}.
+
+Definition addMultiplySpecRule :=
+  {{ let%read st := addMultiplySpecSt in
+     match st with
+     | State__Fetch => addMultiplySpecFetch
+     | State__Decode => addMultiplySpecDecode
+     | State__Execute => addMultiplySpecExecute
+     end
+  }}.
+
+Instance addMultiplySpecCircuit : Circuit :=
+  {|
+    mkCircuit := mkAddMultiplySpec;
+    circuitCall m :=
+      match m with
+      | Spec__DeqIReq => addMultiplySpecDeqIReq
+      | Spec__EnqIResp resp => addMultiplySpecEnqIResp resp
+      | Spec__Rule => addMultiplySpecRule
+      end;
+    circuitTrace := addMultiplySpecTrace
+  |}.
+
+(* Names of RISC-V-like registers *)
+Definition x0 := 3`0%bv.
+Definition x1 := 3`1%bv.
+Definition x2 := 3`2%bv.
+Definition x3 := 3`3%bv.
+Definition x4 := 3`4%bv.
+Definition x5 := 3`5%bv.
+Definition x6 := 3`6%bv.
+Definition x7 := 3`7%bv.
+
+(* Notation for RISC-V-like instructions *)
+Declare Scope asm_scope.
+Delimit Scope asm_scope with asm.
+
+Notation "'addi' rd , rs1 , imm" := (Addi rd rs1 imm)%bv (at level 0) : asm_scope.
+Notation "'li' rd , imm" := (Addi rd 3`0 imm)%bv (at level 0) : asm_scope.
+Notation "'mv' rd , rs" := (Addi rd rs 0)%bv (at level 0) : asm_scope.
+Notation "'add' rd , rs1 , rs2" := (Add rd rs1 rs2)%bv (at level 0) : asm_scope.
+Notation "'muli' rd , imm , rs2" := (Muli rd imm rs2)%bv (at level 0) : asm_scope.
+Notation "'nop'" := Nop (at level 0) : asm_scope.
+
+(* Execute a single instruction until completion *)
+Definition executeOneInstr (fuel : nat) (instr : Instr) (st : AddMultiply) : AddMultiply :=
+  (* Fetch stage: send PC to instruction memory *)
+  let st1 := circuitSteps addMultiplyCircuit [Rule; DeqIReq; EnqIResp instr] st in
+  (* Decode stage *)
+  let st2 := circuitStep addMultiplyCircuit Rule st1 in
+  (* Execute stage - may take multiple cycles *)
+  let fix executeUntilFetch (fuel : nat) (st : AddMultiply) : AddMultiply :=
+    match fuel with
+    | 0 => st
+    | S fuel' =>
+        let st' := circuitStep addMultiplyCircuit Rule st in
+        if decide (st'.(addMultiplySt) = State__Fetch) then
+          st'
+        else
+          executeUntilFetch fuel' st'
+    end
+  in
+  executeUntilFetch fuel st2.
+
+(* Execute instructions with fuel *)
+Fixpoint execute (instrs : list Instr) (st : AddMultiply) : AddMultiply :=
+  match instrs with
+  | [] => st
+  | instr :: instrs' =>
+      let st' := executeOneInstr 100 instr st in
+      execute instrs' st'
+  end.
+
+(* Extract the specification leakage trace from the series of Methods. *)
+Definition policy__dinstr (dinstr : DInstr) : SpecInstr :=
+  match dinstr with
+  | DNop => SNop
+  | DAdd _ _ _ => SAdd
+  | DMul _ imm _ => SMul imm
+  end.
+
+Definition policy__instr (instr : Instr) : SpecInstr :=
+  match instr with
+  | Nop => SNop
+  | Add rd rs1 rs2 => SAdd
+  | Addi rd rs1 imm => SAdd
+  | Muli rd imm rs2 => SMul imm
+  end.
+
+Definition policy1 (m : Method) : SpecLeakage :=
+  match m with
+  | Rule => Spec__Rule
+  | DeqIReq => Spec__DeqIReq
+  | EnqIResp instr => Spec__EnqIResp (policy__instr instr)
+  end.
+
+Definition policy := map policy1.
+
+Definition instrRel instr sinstr :=
+  Eval cbv delta [ policy__instr ] in
+    sinstr = policy__instr instr.
+
+Definition dinstrRel dinstr sinstr :=
+  Eval cbv delta [ policy__dinstr ] in
+    sinstr = policy__dinstr dinstr.
+
+Definition addMultiplyRel st1 st2 :=
+  rel st1.(addMultiplyM) st2.(addMultiplySpecM)
+  /\ st1.(addMultiplyPc) = st2.(addMultiplySpecPc)
+  /\ st1.(addMultiplySt) = st2.(addMultiplySpecSt)
+  /\ st1.(addMultiplyTrace) = st2.(addMultiplySpecTrace)
+  /\ st1.(addMultiplyToImem) = st2.(addMultiplySpecToImem)
+  /\ fifoLift instrRel st1.(addMultiplyFromImem) st2.(addMultiplySpecFromImem)
+  /\ fifoLift dinstrRel st1.(addMultiplyDInstr) st2.(addMultiplySpecDInstr).
+
+Local Hint Unfold fifoDeq fifoFirst fifoEnq fifoNotEmpty fifoNotFull : core.
+Local Hint Unfold addMultiplyRel : core.
+Local Hint Unfold circuitStep nextState set policy__instr : core.
+Local Hint Unfold addMultiplyFetching addMultiplySpecFetching : core.
+Local Hint Unfold addMultiplyExecuting addMultiplySpecExecuting : core.
+Local Hint Unfold addMultiplyExecuteAdd addMultiplySpecExecuteAdd : core.
+Local Hint Unfold addMultiplyExecuteNop addMultiplySpecExecuteNop : core.
+Local Hint Unfold addMultiplyExecuteMul addMultiplySpecExecuteMul : core.
+
+Local Ltac t0 :=
+  match goal with
+  | H0 : fifoLift ?R ?A1 ?A2,
+      H1 : fifoContents ?A1 = None,
+        H2 : fifoContents ?A2 = None -> False
+    |- _ =>
+      assert (~ fifoLift R A1 A2) by eauto;
+      clear H1 H2
+  | H0 : fifoLift ?R ?A1 ?A2,
+      H1 : fifoContents ?A1 = None -> False,
+        H2 : fifoContents ?A2 = None
+    |- _ =>
+      assert (~ fifoLift R A1 A2) by eauto;
+      clear H1 H2
+  | m : Method |- _ => destruct m
+  | i : Instr |- _ => destruct i
+  | |- context [ decide _ ] => case_decide
+  | |- context [ bool_decide _ ] => case_bool_decide
+  | H : _ /\ _ |- _ => propositional
+  | |- _ /\ _ => propositional
+  | _ => try solve [ equality | eauto 8 ]; progress simplify
+  end.
+
+Local Ltac t := repeat t0.
+
+Lemma deqOk : addMultiplyDeqIReq ⪯ addMultiplySpecDeqIReq : addMultiplyRel.
+Proof.
+  cbv [ simulates addMultiplyDeqIReq addMultiplySpecDeqIReq ]; t.
+Qed.
+
+Lemma enqOk : forall resp,
+    addMultiplyEnqIResp resp ⪯ addMultiplySpecEnqIResp (policy__instr resp) : addMultiplyRel.
+Proof.
+  cbv [ simulates addMultiplyEnqIResp addMultiplySpecEnqIResp ]; t.
+Qed.
+
+Lemma fetchOk : addMultiplyFetch ⪯ addMultiplySpecFetch : addMultiplyRel.
+Proof.
+  cbv [ simulates addMultiplyFetch addMultiplySpecFetch ]; t.
+Qed.
+
+Local Hint Resolve fetchOk : core.
+
+Lemma ruleOk : addMultiplyRule ⪯ addMultiplySpecRule : addMultiplyRel. Admitted.
+
+Local Hint Resolve ruleOk deqOk enqOk : core.
+
+Lemma simOk : addMultiplyCircuit ∼ addMultiplySpecCircuit : policy1 ; addMultiplyRel.
+Proof.
+  cbv [ circuitSimulates ]; t.
+Qed.
+
+Local Hint Resolve simOk : core.
+
+Theorem constantTimeOk : constantTime addMultiplyCircuit policy.
+  apply circuitConstantTime with
+    (c2 := addMultiplySpecCircuit)
+    (R := addMultiplyRel);
+    t.
+  - cbv [ rel ]; t.
+  - cbv [ fifoLift instrRel ]; t.
+  - cbv [ fifoLift dinstrRel ]; t.
+Qed.
