src/fifo.v
@@ -35,3 +35,31 @@ Arguments mkFifo {_}.
 Arguments fifoEnq {_} (_ _).
 Arguments fifoDeq {_} (_).
 Arguments fifoFirst {_ _} (_).
+
+Definition fifoLift {t1 t2} (rel : t1 -> t2 -> Prop) (fifo1 : Fifo t1) (fifo2 : Fifo t2) :=
+  match fifo1.(fifoContents), fifo2.(fifoContents) with
+  | Some v1, Some v2 => rel v1 v2
+  | None, None => True
+  | _, _ => False
+  end.
+
+(* Hints about fifoLift. *)
+Lemma hintFifoLift1 {t1 t2} : forall (q1 : Fifo t1) (q2 : Fifo t2) rel,
+    q1.(fifoContents) = None ->
+    q2.(fifoContents) <> None ->
+    ~ fifoLift rel q1 q2.
+Proof.
+  cbv [ fifoLift] in *; simplify.
+  repeat case_match; equality.
+Qed.
+
+Lemma hintFifoLift2 {t1 t2} : forall (q1 : Fifo t1) (q2 : Fifo t2) rel,
+    q1.(fifoContents) <> None ->
+    q2.(fifoContents) = None ->
+    ~ fifoLift rel q1 q2.
+Proof.
+  cbv [ fifoLift] in *; simplify.
+  repeat case_match; equality.
+Qed.
+
+Global Hint Resolve hintFifoLift1 hintFifoLift2 : core.
